theories/Substitution/Introductions/Poly.v
@@ -1,9 +1,9 @@
 From Coq Require Import ssrbool.
 From LogRel.AutoSubst Require Import core unscoped Ast Extra.
-From LogRel Require Import Utils BasicAst Notations Context NormalForms Weakening
-  GenericTyping LogicalRelation Validity.
-From LogRel.LogicalRelation Require Import Escape Reflexivity Neutral Weakening Irrelevance.
-From LogRel.Substitution Require Import Irrelevance Properties.
+From LogRel Require Import Utils BasicAst Notations LContexts Context NormalForms Weakening
+  GenericTyping Monad LogicalRelation Validity.
+From LogRel.LogicalRelation Require Import Escape Reflexivity Neutral Weakening Monotonicity Irrelevance.
+From LogRel.Substitution Require Import Irrelevance Properties Monotonicity.
 From LogRel.Substitution.Introductions Require Import Universe.
 
 Set Universe Polymorphism.
@@ -28,191 +28,313 @@ Section PolyValidity.
 
   Context `{GenericTypingProperties}.
 
-  Lemma mkPolyRed {Γ l A B} (wfΓ : [|-Γ])
-    (RA : forall Δ (ρ : Δ ≤ Γ) (wfΔ : [|- Δ]), [Δ ||-<l> A⟨ρ⟩]) 
-    (RB : forall Δ a (ρ : Δ ≤ Γ) (wfΔ : [|- Δ]), [Δ ||-<l> a : _ | RA Δ ρ wfΔ] -> [Δ ||-<l> B[a .: ρ >> tRel]])
-    (RBext : forall Δ a b (ρ : Δ ≤ Γ) (wfΔ : [|- Δ]) (Ra : [Δ ||-<l> a : _ | RA Δ ρ wfΔ]),
-      [Δ ||-<l> b : _ | RA Δ ρ wfΔ] ->
-      [Δ ||-<l> a ≅ b : _ | RA Δ ρ wfΔ] -> [Δ ||-<l> B[a .: ρ >> tRel] ≅ B[b .: ρ >> tRel] | RB Δ a ρ wfΔ Ra]) :
-    PolyRed Γ l A B.
+  Lemma mkPolyRed {Γ wl l A B} (wfΓ : [|-Γ]< wl >)
+    (RA : forall Δ wl' (ρ : Δ ≤ Γ) (f : wl' ≤ε wl) (wfΔ : [|- Δ]< wl' >), [Δ ||-<l> A⟨ρ⟩]< wl' >)
+    (RB : forall Δ a wl' (ρ : Δ ≤ Γ) (f : wl' ≤ε wl) (wfΔ : [|- Δ]< wl' >) (Ha : [Δ ||-<l> a : _ | RA Δ wl' ρ f wfΔ]< wl' >),
+        W[Δ ||-<l> B[a .: ρ >> tRel]]< wl' >)
+    (RBext : forall Δ a b wl' (ρ : Δ ≤ Γ) (f : wl' ≤ε wl) (wfΔ : [|- Δ]< wl' >)
+                    (Ra : [Δ ||-<l> a : _ | RA Δ wl' ρ f wfΔ]< wl' >)
+                    (Rb : [Δ ||-<l> b : _ | RA Δ wl' ρ f wfΔ]< wl' >)
+                    (Req: [Δ ||-<l> a ≅ b : _ | RA Δ wl' ρ f wfΔ]< wl' >),
+                    W[Δ ||-<l> B[a .: ρ >> tRel] ≅ B[b .: ρ >> tRel] | RB Δ a wl' ρ f wfΔ Ra]< wl' >) :
+    PolyRed wl Γ l A B.
   Proof.
-    assert [Γ |- A] by (eapply escape; now eapply instKripke).
+    assert [Γ |- A]< wl > by (eapply escape ; now eapply instKripke').
     unshelve econstructor; tea.
-    unshelve epose proof (RB _ (tRel 0) (@wk1 Γ A) _ _).
-    + gen_typing.
-    + eapply var0; tea; now rewrite wk1_ren_on.
-    + enough (B = B[tRel 0 .: @wk1 Γ A >> tRel]) as -> by now escape.
-      setoid_rewrite wk1_ren; rewrite scons_eta'; now asimpl.
+    - intros ; now eapply RB.
+    - cbn ; intros.
+      now eapply RB.
+    - intros ; eapply RBext ; [exact ha |..] ; eassumption.
+    - unshelve epose proof (X := RB _ (tRel 0) wl (@wk1 Γ A) (wfLCon_le_id _) _ _).
+      + now gen_typing.
+      + eapply var0; tea ; now rewrite wk1_ren_on .
+      + enough (B = B[tRel 0 .: @wk1 Γ A >> tRel]) as ->.  
+        2: setoid_rewrite wk1_ren; rewrite scons_eta'; now asimpl.
+        now Wescape.
+    - cbn in * ; intros.
+      now eapply RBext.
   Qed.
 
-  Lemma mkPolyRed' {Γ l A B} (RA : [Γ ||-<l> A]) 
-    (RB : forall Δ a (ρ : Δ ≤ Γ) (wfΔ : [|- Δ]), [Δ ||-<l> a : _ | wk ρ wfΔ RA] -> [Δ ||-<l> B[a .: ρ >> tRel]])
-    (RBext : forall Δ a b (ρ : Δ ≤ Γ) (wfΔ : [|- Δ]) (Ra : [Δ ||-<l> a : _ | wk ρ wfΔ RA]),
-      [Δ ||-<l> b : _ | wk ρ wfΔ RA] ->
-      [Δ ||-<l> a ≅ b : _ | wk ρ wfΔ RA] -> [Δ ||-<l> B[a .: ρ >> tRel] ≅ B[b .: ρ >> tRel] | RB Δ a ρ wfΔ Ra]) :
-    PolyRed Γ l A B.
+  Lemma mkPolyRed' {Γ wl l A B} (RA : [Γ ||-<l> A]< wl >) 
+    (RB : forall Δ a wl' (ρ : Δ ≤ Γ) (f : wl' ≤ε wl) (wfΔ : [|- Δ]< wl' >),
+        [Δ ||-<l> a : _ | wk_Ltrans ρ f wfΔ RA]< wl' > -> W[Δ ||-<l> B[a .: ρ >> tRel]]< wl' >)
+    (RBext : forall Δ a b wl' (ρ : Δ ≤ Γ) (f : wl' ≤ε wl) (wfΔ : [|- Δ]< wl' >) (Ra : [Δ ||-<l> a : _ | wk_Ltrans ρ f wfΔ RA]< wl' >),
+      [Δ ||-<l> b : _ | wk_Ltrans ρ f wfΔ RA]< wl' > ->
+      [Δ ||-<l> a ≅ b : _ | wk_Ltrans ρ f wfΔ RA]< wl' > ->
+      W[Δ ||-<l> B[a .: ρ >> tRel] ≅ B[b .: ρ >> tRel] | RB Δ a wl' ρ f wfΔ Ra]< wl' >) :
+    PolyRed wl Γ l A B.
   Proof.
     unshelve eapply mkPolyRed; tea.
-    escape; gen_typing.
+    3: escape; gen_typing.
+    1: intros ; now eapply wk_Ltrans.
+    - intros ; now eapply RB.
+    - intros ; now eapply RBext.
   Qed.
 
 
-  Lemma polyCodSubstRed {Γ l F G} (RF : [Γ ||-<l> F]) : 
-    PolyRed Γ l F G -> forall t, [Γ ||-<l> t : _ | RF] -> [Γ ||-<l> G[t..]].
+  Lemma polyCodSubstRed {Γ wl l F G} (RF : [Γ ||-<l> F]< wl >) : 
+    PolyRed wl Γ l F G -> forall t, [Γ ||-<l> t : _ | RF]< wl > -> W[Γ ||-<l> G[t..]]< wl >.
   Proof.
     intros PFG ??. 
-    escape. assert (wfΓ : [|- Γ]) by gen_typing.
+    escape. assert (wfΓ : [|- Γ]< wl >) by gen_typing.
     erewrite <- subst_wk_id_tail.
-    eapply (PolyRed.posRed PFG wk_id wfΓ).
-    irrelevance.
+    unshelve econstructor.
+    - unshelve eapply (PolyRed.posTree PFG wk_id (wfLCon_le_id _) wfΓ).
+      2: irrelevance. 
+    - now eapply (PolyRed.posRed PFG wk_id _ wfΓ).
   Qed.
 
-  Lemma polyCodSubstExtRed {Γ l F G} (RF : [Γ ||-<l> F]) (PFG : PolyRed Γ l F G) (RG := polyCodSubstRed RF PFG) :
-    forall t u (Rt : [Γ ||-<l> t : _ | RF]), [Γ ||-<l> u : _ | RF] -> [Γ ||-<l> t ≅ u : _ | RF] -> 
-    [Γ ||-<l> G[t..] ≅ G[u..]| RG t Rt].
+  Lemma polyCodSubstExtRed {Γ wl l F G} (RF : [Γ ||-<l> F]< wl >) (PFG : PolyRed wl Γ l F G) (RG := polyCodSubstRed RF PFG) :
+    forall t u (Rt : [Γ ||-<l> t : _ | RF]< wl >), [Γ ||-<l> u : _ | RF]< wl > -> [Γ ||-<l> t ≅ u : _ | RF]< wl > -> 
+    W[Γ ||-<l> G[t..] ≅ G[u..]| RG t Rt]< wl >.
   Proof.
-    intros. escape. assert (wfΓ : [|- Γ]) by gen_typing.
-    irrelevance0; erewrite <- subst_wk_id_tail; [reflexivity|].
-    unshelve eapply (PolyRed.posExt PFG wk_id wfΓ); irrelevance.
+    intros. escape. assert (wfΓ : [|- Γ]< wl >) by gen_typing.
+    unshelve Wirrelevance0 ; [eassumption | ..].
+    3: erewrite <- subst_wk_id_tail; reflexivity.
+    1,2: unshelve econstructor.
+    - eapply DTree_fusion.
+      + eapply (PolyRed.posTree (a := t) PFG wk_id (wfLCon_le_id _) wfΓ).
+        irrelevance.
+      + eapply (PolyRed.posTree (a := u) PFG wk_id (wfLCon_le_id _) wfΓ).
+        irrelevance.
+    - unshelve eapply (PolyRed.posExtTree PFG wk_id (wfLCon_le_id _) wfΓ).
+      5: irrelevance.
+      1,2: now irrelevance.
+    - intros.
+      now eapply (PolyRed.posRed PFG wk_id _ wfΓ), over_tree_fusion_l.
+    - intros ; irrelevanceRefl.
+      erewrite <- subst_wk_id_tail.
+      unshelve eapply (PolyRed.posExt PFG wk_id (wfLCon_le_id _) wfΓ).
+      1,3,4: irrelevance.
+      3: eassumption.
+      1: eapply over_tree_fusion_l ; exact Hover.
+      1: eapply over_tree_fusion_r ; exact Hover.
   Qed.  
 
 
-  Lemma polyRedId {Γ l F G} : PolyRed Γ l F G -> [Γ ||-<l> F] × [Γ ,, F ||-<l> G].
+  Lemma polyRedId {Γ wl l F G} : PolyRed wl Γ l F G -> [Γ ||-<l> F]< wl > × W[Γ ,, F ||-<l> G]< wl >.
   Proof.
-    intros [?? RF RG]; split.
-    -  rewrite <- (wk_id_ren_on Γ F). eapply RF; gen_typing.
+    intros [?? RF ? RG]; split.
+    - rewrite <- (wk_id_ren_on Γ F).
+      eapply RF ; [now eapply wfLCon_le_id | now gen_typing].
     - replace G with G[tRel 0 .: @wk1 Γ F >> tRel].
       2: bsimpl; rewrite scons_eta'; now asimpl.
-      eapply RG. eapply var0; tea; now bsimpl.
-      Unshelve. gen_typing.
-  Qed.
+      econstructor ; eapply RG.
+      Unshelve.
+      + now eapply wfLCon_le_id.
+      + now gen_typing.
+      + eapply var0; tea; now bsimpl.
+  Defined.
 
-  Lemma polyRedEqId {Γ l F F' G G'} (PFG : PolyRed Γ l F G) (RFG := polyRedId PFG) :
-    PolyRedEq PFG F' G' -> [Γ ||-<l> F ≅ F' | fst RFG] × [Γ ,, F ||-<l> G ≅ G' | snd RFG].
+  Lemma polyRedEqId {Γ wl l F F' G G'} (PFG : PolyRed wl Γ l F G) (RFG := polyRedId PFG) :
+    PolyRedEq PFG F' G' -> [Γ ||-<l> F ≅ F' | fst RFG]< wl > × W[Γ ,, F ||-<l> G ≅ G' | snd RFG]< wl >.
   Proof.
-    intros [RFF' RGG']; destruct RFG; escape; split.
+    intros [RFF' ? RGG']; destruct RFG; escape; split.
     - rewrite <- (wk_id_ren_on Γ F'); irrelevance0.
-      2: unshelve eapply RFF'; gen_typing.
-      apply wk_id_ren_on.
+      2: unshelve eapply RFF'; [ now eapply wfLCon_le_id | gen_typing].
+      now apply wk_id_ren_on.
     - replace G' with G'[tRel 0 .: @wk1 Γ F >> tRel].
       2: bsimpl; rewrite scons_eta'; now asimpl.
-      irrelevance0.
-      2: eapply RGG'.
-      bsimpl; rewrite scons_eta'; now asimpl.
-      Unshelve. 1: gen_typing.
-      eapply var0; tea; now bsimpl.
+      unshelve econstructor ; intros.
+      1: eapply DTree_fusion ; [eapply (PolyRedPack.posTree PFG (wk1 F)) | eapply posTree].
+      1,2: eapply var0 ; tea.
+      1: now bsimpl.
+      2: irrelevance0.
+      3: eapply RGG'. 
+      2: bsimpl; rewrite scons_eta'; now asimpl.
+      Unshelve.
+      2: eapply over_tree_fusion_r ; exact Hover'.
+      2,4: now eapply wfLCon_le_id.
+      2,3: now gen_typing.
+      1: now bsimpl.
+      eapply over_tree_fusion_l ; exact Hover'. 
   Qed.
 
-  Lemma polyRedSubst {Γ l A B t} (PAB : PolyRed Γ l A B) 
-    (Rt : forall Δ a (ρ : Δ ≤ Γ) (wfΔ : [|-Δ]), 
-      [Δ ||-<l> a : _ | PolyRed.shpRed PAB ρ wfΔ] ->
-      [Δ ||-<l> t[a .: ρ >> tRel] : _ | PolyRed.shpRed PAB ρ wfΔ ])
-    (Rtext : forall Δ a b (ρ : Δ ≤ Γ) (wfΔ : [|-Δ]), 
-      [Δ ||-<l> a : _ | PolyRed.shpRed PAB ρ wfΔ] ->
-      [Δ ||-<l> b : _ | PolyRed.shpRed PAB ρ wfΔ] ->
-      [Δ ||-<l> a ≅ b : _ | PolyRed.shpRed PAB ρ wfΔ] ->
-      [Δ ||-<l> t[a .: ρ >> tRel] ≅ t[b .: ρ >> tRel] : _ | PolyRed.shpRed PAB ρ wfΔ ])
-    : PolyRed Γ l A B[t]⇑.
+  Lemma polyRedSubst {wl Γ l A B t} (PAB : PolyRed wl Γ l A B) 
+    (Rt : forall Δ wl' a (ρ : Δ ≤ Γ) (f : wl' ≤ε wl) (wfΔ : [|-Δ]< wl' >), 
+      [Δ ||-<l> a : _ | PolyRed.shpRed PAB ρ f wfΔ]< wl' > ->
+      [Δ ||-<l> t[a .: ρ >> tRel] : _ | PolyRed.shpRed PAB ρ f wfΔ ]< wl' >)
+    (Rtext : forall Δ wl' a b (ρ : Δ ≤ Γ) (f : wl' ≤ε wl) (wfΔ : [|-Δ]< wl' >), 
+      [Δ ||-<l> a : _ | PolyRed.shpRed PAB ρ f wfΔ]< wl' > ->
+      [Δ ||-<l> b : _ | PolyRed.shpRed PAB ρ f wfΔ]< wl' > ->
+      [Δ ||-<l> a ≅ b : _ | PolyRed.shpRed PAB ρ f wfΔ]< wl' > ->
+      [Δ ||-<l> t[a .: ρ >> tRel] ≅ t[b .: ρ >> tRel] : _ | PolyRed.shpRed PAB ρ f wfΔ ]< wl' >)
+    : PolyRed wl Γ l A B[t]⇑.
   Proof.
-    destruct PAB; opector; tea.
-    + intros; rewrite liftSubst_scons_eq.
-      unshelve eapply posRed; tea; eapply Rt; now irrelevanceRefl.
-    + unshelve epose proof (posRed _ t (@wk1 Γ A) _ _).
-      - escape; gen_typing.
-      - replace t with t[tRel 0 .: @wk1 Γ A >> tRel].
-        2:{ bsimpl; rewrite scons_eta'; now asimpl. }
-        eapply Rt.
-        eapply var0; tea; now rewrite wk1_ren_on.
-      - escape. 
-        replace (B[_]) with B[t .: @wk1 Γ A >> tRel]; tea.
-        now setoid_rewrite wk1_ren.
-    + intros; irrelevance0; rewrite liftSubst_scons_eq;[reflexivity|].
-      unshelve eapply posExt; tea; eapply Rt + eapply Rtext; now irrelevanceRefl.
+    destruct PAB.
+    unshelve econstructor ; [tea | | | | tea |tea | ] ; cbn in *.
+    1:{ intros ; eapply (posTree Δ k' t[a .: ρ >> tRel] ρ f).
+      1: eapply Rt ; irrelevanceRefl ; eassumption. }
+    1:{ intros; rewrite liftSubst_scons_eq.
+        pose proof (X1 := over_tree_le Ho).
+        pose proof (X2 := wfLCon_le_trans X1 f).
+        unshelve eapply posRed ; [ | exact f | eassumption |.. ].
+        1: eapply Rt ; irrelevanceRefl ; eassumption.
+        exact Ho. }
+    2:{ pattern wl ; eapply split_to_over_tree.
+        + intros ; now eapply wft_ϝ.
+        + intros wl' Hover.
+          unshelve epose proof (posRed _ t _ (@wk1 Γ A) (wfLCon_le_id _) _ _ _ Hover).
+          * escape; gen_typing.
+          * replace t with t[tRel 0 .: @wk1 Γ A >> tRel].
+            2:{ bsimpl; rewrite scons_eta'; now asimpl. }
+            eapply Rt.
+            eapply var0; tea; now rewrite wk1_ren_on.
+          * escape.
+            replace (B[_]) with B[t .: @wk1 Γ A >> tRel]; tea.
+            now setoid_rewrite wk1_ren. }
+    2:{ intros; irrelevance0; rewrite liftSubst_scons_eq;[reflexivity|].
+        unshelve eapply posExt ; cbn in *.
+        2,3: eassumption.
+        1,3: eapply Rt ; now irrelevanceRefl.
+        2: eapply Rtext ; now irrelevanceRefl.
+        1,2: eassumption.
+        exact Hoeq. }
   Qed.
 
-  Lemma polyRedEqSubst {Γ l A B t u} (PAB : PolyRed Γ l A B) 
-    (Rt : forall Δ a (ρ : Δ ≤ Γ) (wfΔ : [|-Δ]), 
-      [Δ ||-<l> a : _ | PolyRed.shpRed PAB ρ wfΔ] ->
-      [Δ ||-<l> t[a .: ρ >> tRel] : _ | PolyRed.shpRed PAB ρ wfΔ ])
-    (Ru : forall Δ a (ρ : Δ ≤ Γ) (wfΔ : [|-Δ]), 
-      [Δ ||-<l> a : _ | PolyRed.shpRed PAB ρ wfΔ] ->
-      [Δ ||-<l> u[a .: ρ >> tRel] : _ | PolyRed.shpRed PAB ρ wfΔ ])
-    (Rtu : forall Δ a b (ρ : Δ ≤ Γ) (wfΔ : [|-Δ]), 
-      [Δ ||-<l> a : _ | PolyRed.shpRed PAB ρ wfΔ] ->
-      [Δ ||-<l> b : _ | PolyRed.shpRed PAB ρ wfΔ] ->
-      [Δ ||-<l> a ≅ b : _ | PolyRed.shpRed PAB ρ wfΔ] ->
-      [Δ ||-<l> t[a .: ρ >> tRel] ≅ u[b .: ρ >> tRel] : _ | PolyRed.shpRed PAB ρ wfΔ ])
-    (PABt : PolyRed Γ l A B[t]⇑)
+  Lemma polyRedEqSubst {Γ wl l A B t u} (PAB : PolyRed wl Γ l A B) 
+    (Rt : forall Δ wl' a (ρ : Δ ≤ Γ) (f : wl' ≤ε wl) (wfΔ : [|-Δ]< wl' >), 
+        [Δ ||-<l> a : _ | PolyRed.shpRed PAB ρ f wfΔ]< wl' > ->
+        [Δ ||-<l> t[a .: ρ >> tRel] : _ | PolyRed.shpRed PAB ρ f wfΔ ]< wl' >)
+    (Ru : forall Δ wl' a (ρ : Δ ≤ Γ) (f : wl' ≤ε wl) (wfΔ : [|-Δ]< wl' >), 
+        [Δ ||-<l> a : _ | PolyRed.shpRed PAB ρ f wfΔ]< wl' > ->
+        [Δ ||-<l> u[a .: ρ >> tRel] : _ | PolyRed.shpRed PAB ρ f wfΔ ]< wl' >)
+    (Rtu : forall Δ wl' a b (ρ : Δ ≤ Γ) (f : wl' ≤ε wl) (wfΔ : [|-Δ]< wl' >), 
+        [Δ ||-<l> a : _ | PolyRed.shpRed PAB ρ f wfΔ]< wl' > ->
+        [Δ ||-<l> b : _ | PolyRed.shpRed PAB ρ f wfΔ]< wl' > ->
+        [Δ ||-<l> a ≅ b : _ | PolyRed.shpRed PAB ρ f wfΔ]< wl' > ->
+        [Δ ||-<l> t[a .: ρ >> tRel] ≅ u[b .: ρ >> tRel] : _ | PolyRed.shpRed PAB ρ f wfΔ ]< wl' >)
+    (PABt : PolyRed wl Γ l A B[t]⇑)
     : PolyRedEq PABt A B[u]⇑.
   Proof.
-    constructor.
-    - intros; eapply reflLRTyEq.
-    - intros; irrelevance0; rewrite liftSubst_scons_eq; [reflexivity|].
-      unshelve eapply PolyRed.posExt; cycle 1; tea.
-      + eapply Rt; now irrelevanceRefl.
-      + eapply Ru; now irrelevanceRefl.
-      + eapply Rtu; try eapply reflLRTmEq; now irrelevanceRefl.
+    unshelve econstructor.
+    2: intros; now eapply reflLRTyEq.
+    2:{ intros; irrelevance0; rewrite liftSubst_scons_eq; [reflexivity|].
+        unshelve eapply PolyRed.posExt; cycle 1.
+        4,5: eassumption.
+        3: eapply Rt; now irrelevanceRefl.
+        2: eapply Ru; now irrelevanceRefl.
+        2: eapply Rtu; try eapply reflLRTmEq; now irrelevanceRefl.
+        3: eapply over_tree_fusion_r ; exact Ho'.
+        1: do 2 eapply over_tree_fusion_l ; exact Ho'.
+        eapply over_tree_fusion_r, over_tree_fusion_l ; exact Ho'.
+    }
   Qed.
   
-  Context {l Γ F G} (VΓ : [||-v Γ])
-    (VF : [Γ ||-v< l > F | VΓ ])
-    (VG : [Γ ,, F ||-v< l > G | validSnoc VΓ VF]).
+  Context {l wl Γ F G} (VΓ : [||-v Γ]< wl >)
+    (VF : [Γ ||-v< l > F | VΓ ]< wl >)
+    (VG : [Γ ,, F ||-v< l > G | validSnoc' VΓ VF]< wl >).
 
-  Context {Δ σ} (tΔ : [ |-[ ta ] Δ]) (Vσ : [VΓ | Δ ||-v σ : _ | tΔ]).
+  Context {Δ σ wl' f} (tΔ : [ |-[ ta ] Δ]< wl' >) (Vσ : [VΓ | Δ ||-v σ : _ | tΔ | f]< wl >).
   
-  Lemma substPolyRed : PolyRed Δ l F[σ] G[up_term_term σ].
+  Lemma substPolyRed : WPolyRed wl' Δ l F[σ] G[up_term_term σ].
   Proof.
     pose proof (Vuσ := liftSubstS' VF Vσ).
-    instValid Vσ; instValid Vuσ; escape.
-    unshelve econstructor; tea.
-    - intros; now eapply wk.
-    - cbn; intros ?? ρ wfΔ' ha.
-      rewrite eq_subst_2.
-      pose proof (Vawkσ := consWkSubstS VF ρ wfΔ' Vσ ha).
-      now instValid Vawkσ.
-    - cbn; intros ??? ρ wfΔ' ha hb hab.
+    instValid Vσ; instValid Vuσ; Wescape.
+    exists (DTree_fusion _ (WT _ RVF) (WT _ RVG)).
+    intros wl'' Hover.
+    pose proof (HoF := over_tree_fusion_l Hover).
+    pose proof (HoG := over_tree_fusion_r Hover).
+    unshelve econstructor.
+    5,6: now eapply wft_Ltrans ; [ eapply over_tree_le | eassumption].
+    1: intros; eapply wk ; [eassumption | eapply RVF, le_over_tree ; eassumption].
+    2:{ cbn; intros ??? ρ f' wfΔ' ha wl''' Hover'.
+        rewrite eq_subst_2.
+        unshelve eapply (validTy VG).
+        3: eassumption.
+        1: exact (f' •ε (over_tree_le Hover) •ε f).
+        eapply consWkSubstS.
+        1: eapply subst_Ltrans ; eassumption.
+        1: now eapply TmLogtoW.
+        exact Hover'.
+    }
+    2:{ cbn; intros ???? ρ f' wfΔ' ha hb hab wl''' Hoa Hob Hoeq.
       irrelevance0; rewrite eq_subst_2.
       1: reflexivity.
-      pose proof (Vawkσ := consWkSubstS VF ρ wfΔ' Vσ ha).
-      pose proof (Vbwkσ := consWkSubstS VF ρ wfΔ' Vσ hb).
-      epose proof (Vabwkσ := consWkSubstSEq' VF Vσ (reflSubst _ _ Vσ) ρ wfΔ' ha hab).
-      now instAllValid Vawkσ Vbwkσ Vabwkσ.
-  Qed.
+      eapply (validTyExt VG).
+      exact Hoeq.
+    }
+    Unshelve.
+    2: exact Hoa.
+    2:eapply (consWkSubstS VF ρ) ; [ eapply subst_Ltrans ; eassumption | ].
+    2: now eapply TmLogtoW.
+    2: unshelve eapply (consWkSubstSEq' VF _ _ ρ).
+    3: now eapply TmEqLogtoW.
+    2: now eapply eqsubst_Ltrans, (reflSubst _ _ _ Vσ).
+    Unshelve.
+    all: eapply wfc_Ltrans ; [| eassumption].
+    all: exact (f' •ε over_tree_le Hover).
+  Qed. 
 
-  Lemma substEqPolyRedEq {F' G'} (VF' : [Γ ||-v< l > F' | VΓ ])
-    (VG' : [Γ ,, F' ||-v< l > G' | validSnoc VΓ VF'])
-    (VFF' : [Γ ||-v< l > F ≅ F' | VΓ | VF])
-    (VGG' : [Γ ,, F ||-v< l > G ≅ G' | validSnoc VΓ VF | VG])
-    : PolyRedEq substPolyRed F'[σ] G'[up_term_term σ].
+  Lemma substEqPolyRedEq {F' G'} (VF' : [Γ ||-v< l > F' | VΓ ]< wl >)
+    (VG' : [Γ ,, F' ||-v< l > G' | validSnoc' VΓ VF']< wl >)
+    (VFF' : [Γ ||-v< l > F ≅ F' | VΓ | VF]< wl >)
+    (VGG' : [Γ ,, F ||-v< l > G ≅ G' | validSnoc' VΓ VF | VG]< wl >)
+    : WPolyRedEq substPolyRed F'[σ] G'[up_term_term σ].
   Proof.
     instValid Vσ.
-    unshelve econstructor.
-    - intros; irrelevanceRefl; now unshelve eapply wkEq.
-    - intros ?? ρ wfΔ' ha; irrelevance0; rewrite eq_subst_2.
-      1: reflexivity.
-      unshelve epose proof (Vabwkσ := consWkSubstSEq' VF Vσ (reflSubst _ _ Vσ) ρ wfΔ' ha _).
-      2: now eapply reflLRTmEq.
-      unshelve eapply validTyEq; cycle 2; tea. 
-      now eapply consWkSubstS.
-  Qed.
+    unshelve econstructor ; [ | unshelve econstructor].
+    3:{ intros; irrelevanceRefl.
+        unshelve eapply wkEq ; [eassumption | eapply RVF | eapply RVFF' ].
+        all: eapply le_over_tree ; [eassumption | ].
+        eapply over_tree_fusion_l ; exact Ho'.
+        eapply over_tree_fusion_r ; exact Ho'.
+    }
+    2:{ intros ??? ρ f' wfΔ' ha wl'' Hoa Hoeq.
+        irrelevance0; rewrite eq_subst_2.
+        1: reflexivity.
+        unshelve epose proof (Vabwkσ := consWkSubstSEq' VF _ _ ρ wfΔ' _).
+        7: unshelve eapply subst_Ltrans ; [ .. | exact Vσ].
+        6: unshelve eapply eqsubst_Ltrans ; exact (reflSubst _ _ _ Vσ).
+        6: eapply TmLogtoW ; exact ha.
+        2: eapply wfc_Ltrans ; [ | eassumption ].
+        2,3: exact (f' •ε over_tree_le Ho).
+        2: unshelve eapply validTyEq ; [ | | | eassumption | ..].
+        4,7: eassumption.
+        2: exact (f' •ε over_tree_le Ho •ε f).
+        2: eapply consWkSubstS ; [ eapply subst_Ltrans ; eassumption | ].
+        2: eapply TmLogtoW ; exact ha.
+        2: eapply over_tree_fusion_l ; exact Hoeq.
+        2: eapply over_tree_fusion_r ; exact Hoeq.
+        Unshelve.
+        1: eassumption.
+        eapply wfc_Ltrans ; [ exact (f' •ε over_tree_le Ho) | eassumption ].
+    }
+Qed.        
 
-  Context {σ'} (Vσ' : [VΓ | Δ ||-v σ' : _ | tΔ]) (Vσσ' : [VΓ | Δ ||-v σ ≅ σ' : _ | tΔ | Vσ]).
+  Context {σ'} (Vσ' : [VΓ | Δ ||-v σ' : _ | tΔ | f]< wl >) (Vσσ' : [VΓ | Δ ||-v σ ≅ σ' : _ | tΔ | Vσ| f]< wl >).
 
-  Lemma substPolyRedEq : PolyRedEq substPolyRed F[σ'] G[up_term_term σ'].
+  Lemma substPolyRedEq : WPolyRedEq substPolyRed F[σ'] G[up_term_term σ'].
   Proof.
     instAllValid Vσ Vσ' Vσσ'.
-    unshelve econstructor.
-    - intros; irrelevanceRefl; now eapply wkEq.
-    - intros ?? ρ wfΔ' ha; irrelevance0; rewrite eq_subst_2.
-      1: reflexivity.
-      unshelve epose proof (Vabwkσ := consWkSubstSEq' VF Vσ Vσσ' ρ wfΔ' ha _).
-      2: now eapply reflLRTmEq.
-      eapply validTyExt; tea.
-      eapply consWkSubstS; tea.
-      eapply LRTmRedConv; tea.
-      irrelevanceRefl; now eapply wkEq.
-      Unshelve. 1,3,5: tea. now eapply wk.
-  Qed.
+    econstructor ; intros ; unshelve econstructor.
+    2:{ intros; irrelevanceRefl ; eapply wkEq, REVF.
+        eapply le_over_tree, over_tree_fusion_r ; [ eassumption | exact Ho'].
+    }
+    2:{ intros ??? ρ f' wfΔ' ha wl'' Ho'' Hoeq.
+        irrelevance0; rewrite eq_subst_2.
+        1: reflexivity.
+        unshelve eapply (validTyExt VG).
+        3: eassumption.
+        1: exact (f' •ε over_tree_le Ho •ε f).
+        2: eapply over_tree_fusion_l ; exact Hoeq.
+        4: eapply over_tree_fusion_r ; exact Hoeq.
+        1,2: eapply consWkSubstS.
+        1,3: unshelve eapply subst_Ltrans ; [ .. | exact Vσ + exact Vσ'].
+        2: eapply WLRTmRedConv.
+        1,3: eapply TmLogtoW ; exact ha.
+        1: Wirrelevance0 ; [reflexivity | eapply WwkEq_Ltrans ; eassumption].
+        unshelve eapply (consWkSubstSEq' VF).
+        1:unshelve eapply eqsubst_Ltrans ; exact Vσσ'.
+        eapply WreflLRTmEq, TmLogtoW ; exact ha.
+        Unshelve.
+        1,8: eassumption.
+        1: eapply over_tree_fusion_l, le_over_tree ; [ eauto | exact Ho'].
+        1,2: eapply wfc_Ltrans ; [ | eassumption].
+        3: eapply Wwk_Ltrans ; [ | eassumption | eassumption].
+        all: exact (f' •ε over_tree_le Ho).
+    }
+Qed.        
 
 End PolyValidity.
 
